backends/lean/Aeneas/Tactic/Step/InferPost.lean
@@ -1,10 +1,10 @@
 module
 public import Lean
 public import AeneasMeta.Utils
-public import AeneasMeta.Simp.Simp
+public meta import AeneasMeta.Simp.Simp
 public import Mathlib.Tactic.Simproc.ExistsAndEq
 public import Aeneas.Tactic.Solver.Grind.Init
-public import Aeneas.Tactic.Step.Init
+public meta import Aeneas.Tactic.Step.Init
 public section
 
 namespace Aeneas
@@ -18,7 +18,7 @@ open Lean Elab Meta Tactic TacticM
 
     `eliminate` controls which free variables to try clearing from the context before collecting
     escaping variables -/
-def inferPost (goal : MVarId) (eliminate : LocalDecl → Bool := fun _ => true) :
+meta def inferPost (goal : MVarId) (eliminate : LocalDecl → Bool := fun _ => true) :
     TacticM MVarId := withTraceNode `Step (fun _ => do pure m!"inferPost") <| goal.withContext do
   traceGoalWithNode "metavariable context"
   let goalTy ← instantiateMVars (← goal.getType)
